\documentclass[14pt]{article}

% Packages
\usepackage[utf8]{inputenc}
\usepackage[english]{babel}
\usepackage[letterpaper,top=2cm,bottom=2cm,left=2cm,right=2cm,bindingoffset=0mm]{geometry}
\usepackage{amssymb}
\usepackage{amsmath}
\usepackage{tikz}
\usepackage{graphicx}
\usepackage{comment}
\usepackage{rotating}
\usepackage{float}
\usepackage{natbib}
\usepackage{amsthm}
\usepackage{bbm}
\usepackage{thmtools,thm-restate}
\usepackage{hyperref}
%\usepackage{extsizes}
\usepackage[font=footnotesize,labelfont=bf]{caption}

% New Options
\newtheorem{prop}{Proposition}
\newtheorem{definition}{Definition}[section]
\newtheorem*{remark}{Remark}
\newtheorem{lemma}{Lemma}
\declaretheorem{proposition}
\linespread{1.2}
\raggedbottom
\font\reali=msbm10 at 12pt

% New Commands
\newcommand{\real}{\hbox{\reali R}}
\newcommand{\realp}{\hbox{\reali R}_{\scriptscriptstyle +}}
\newcommand{\realpp}{\hbox{\reali R}_{\scriptscriptstyle ++}}
\newcommand{\R}{\mathbb{R}}
\DeclareMathOperator{\E}{\mathbb{E}}


\begin{document}
	
	\large{

\section*{Structural Form}

Assume an economy with two variables: $X_1$ and $X_2$; and two structural shocks: $s_1$ and $s_2$. Law of motions of $X_1$ and $X_2$ has the following process:
\begin{eqnarray}
X_t = B(L)X_{t-1} + As_t
\end{eqnarray}
which is
\begin{eqnarray}
\begin{cases}
X_{1,t} = B_{1,1}(L)X_{1,t-1} + B_{1,2}(L)X_{2,t-1} + A_{1,1}s_{1,t} + A_{1,2}s_{2,t} \\
X_{2,t} = B_{2,1}(L)X_{1,t-1} + B_{2,2}(L)X_{2,t-1} + A_{2,1}s_{1,t} - A_{2,2}s_{2,t}
\end{cases}
\end{eqnarray}
I assume to know exactly the values of matrix $B(L)$ and to only know signs of each element of matrix $A$. Without loss of generality I will assume that each element of $A$ is strictly positive. Objective is to recover from the reduced-form VAR,
\begin{eqnarray}
\begin{cases}
X_{1,t} = B_{1,1}(L)X_{1,t-1} + B_{1,2}(L)X_{2,t-1} + i_{1,t} \\
X_{2,t} = B_{2,1}(L)X_{1,t-1} + B_{2,2}(L)X_{2,t-1} + i_{2,t}
\end{cases}
\end{eqnarray}
structural matrix $A$. In particular, I want to be able to solve the system
\begin{eqnarray}
As_t = i_t
\end{eqnarray}
which is
\begin{eqnarray}
\begin{cases}
A_{1,1}s_{1,t} + A_{1,2}s_{2,t} = i_{1,t} \\
A_{2,1}s_{1,t} - A_{2,2}s_{2,t} = i_{2,t}
\end{cases}
\end{eqnarray}
Since by assumption, $s_t's_t = I_2$, we have that $A'A = i'_t i_t$ which is
\begin{eqnarray}
\begin{pmatrix}
A_{1,1} & A_{1,2} \\
A_{2,1} & A_{2,2}
\end{pmatrix} \begin{pmatrix}
A_{1,1} & A_{2,1} \\
A_{1,2} & A_{2,2}
\end{pmatrix}  = \begin{pmatrix}
\sigma^2_{1,1} & \sigma^2_{1,2} \\
\sigma^2_{1,2} & \sigma^2_{2,2}
\end{pmatrix}
\end{eqnarray}
which is
\begin{eqnarray}
\begin{pmatrix}
A_{1,1}^2 + A_{1,2}^2 & A_{1,1} A_{2,1} + A_{1,2} A_{2,2}  \\
A_{1,1} A_{2,1} + A_{1,2} A_{2,2}  & A_{2,1}^2 + A_{2,2}^2
\end{pmatrix} = \begin{pmatrix}
\sigma^2_{1,1} & \sigma^2_{1,2} \\
\sigma^2_{2,1} & \sigma^2_{2,2}
\end{pmatrix}
\end{eqnarray}
which boils down to the following system,
\begin{eqnarray}
\begin{cases}
A_{1,1}^2 + A_{1,2}^2 = \sigma^2_{1,1} \\
A_{1,1} A_{2,1} + A_{1,2} A_{2,2} = \sigma^2_{1,2} \\
A_{2,1}^2 + A_{2,2}^2 = \sigma^2_{2,2} \\
\end{cases}
\end{eqnarray}
Assume you solve the system by using a standard Cholesky identification where $A_{1,2} = 0$,
\begin{eqnarray}
chol(A) = \begin{pmatrix}
\sigma_{1,1} & 0 \\
\frac{\sigma_{1,2}^2}{\sigma_{1,1}} & \sqrt{\sigma_{2,2}^2 - \Big( \frac{\sigma_{1,2}^2}{\sigma_{1,1}} \Big)^2} \\
\end{pmatrix} = \begin{pmatrix}
c_{1,1} & 0 \\
c_{2,1} & c_{2,2} \\
\end{pmatrix}
\end{eqnarray}
Now, define an orthogonal matrix $D$ which will be used to identify the structural shocks,
\begin{eqnarray}
D = \begin{pmatrix}
\Gamma_{1} & \Gamma_{2} \\
\end{pmatrix} = \begin{pmatrix}
\gamma_{1,1} & \gamma_{1,2} \\
\gamma_{2,1} & \gamma_{2,2} \\
\end{pmatrix} 
\end{eqnarray}
where $D'D = I$. Moreover, impact matrix is now,
\begin{eqnarray}
\begin{pmatrix}
A_{1,1} & A_{1,2} \\
A_{2,1} & A_{2,2}
\end{pmatrix} = \begin{pmatrix}
c_{1,1} \gamma_{1,1} & c_{1,1} \gamma_{1,2} \\
c_{2,1} \gamma_{1,1} + c_{2,2} \gamma_{2,1} & c_{2,1} \gamma_{1,2} + c_{2,2} \gamma_{2,2}
\end{pmatrix}
\end{eqnarray}
which is
\begin{eqnarray}
\begin{pmatrix}
A_{1,1} & A_{1,2} \\
A_{2,1} & A_{2,2}
\end{pmatrix} = \begin{pmatrix}
\sigma_{1,1} \gamma_{1,1} & \sigma_{1,1} \gamma_{1,2} \\
\frac{\sigma_{1,2}^2}{\sigma_{1,1}} \gamma_{1,1} + \sqrt{\sigma_{2,2}^2 - \Big( \frac{\sigma_{1,2}^2}{\sigma_{1,1}} \Big)^2} \gamma_{2,1} & \frac{\sigma_{1,2}^2}{\sigma_{1,1}} \gamma_{1,2} + \sqrt{\sigma_{2,2}^2 - \Big( \frac{\sigma_{1,2}^2}{\sigma_{1,1}} \Big)^2} \gamma_{2,2}
\end{pmatrix}
\end{eqnarray}
%which is
%$$
%\begin{pmatrix}
%A_{1,1} & A_{1,2} \\
%A_{2,1} & A_{2,2}
%\end{pmatrix} = \begin{pmatrix}
%\sigma_{1,1} \gamma_{1,1} & \sigma_{1,1} \gamma_{1,2} \\
%\frac{\sigma_{1,2}^2}{\sigma_{1,1}} \gamma_{1,1} + \sqrt{\sigma_{2,2}^2 - \Big( \frac{\sigma_{1,2}^2}{\sigma_{1,1}} \Big)^2} \sqrt{1 - \gamma_{1,1}^2} & \frac{\sigma_{1,2}^2}{\sigma_{1,1}} \gamma_{1,2} - \sqrt{\sigma_{2,2}^2 - \Big( \frac{\sigma_{1,2}^2}{\sigma_{1,1}} \Big)^2} \sqrt{1 - \gamma_{1,2}^2}
%\end{pmatrix}
%$$
Identification of $s_{1,t}$ is
\begin{eqnarray}\label{eq:problem_Gam1}
\begin{aligned}
\max_{\gamma_{1,1},\gamma_{2,1}} \ \ & \ \sigma_{1,1} \gamma_{1,1} + \delta \Bigg[ \frac{\sigma_{1,2}^2}{\sigma_{1,1}}  \gamma_{1,1} + \sqrt{\sigma_{2,2}^2 - \Big( \frac{\sigma_{1,2}^2}{\sigma_{1,1}} \Big)^2} \gamma_{2,1}   \Bigg] \\
\text{s.t.} \ \ & \ 1 \geq \gamma_{1,1}^2 + \gamma_{2,1}^2
\end{aligned}
\end{eqnarray}
Resetting the problem with Lagrangian function is
\begin{eqnarray}\label{eq:lagrangian}
\begin{aligned}
\max_{\gamma_{1,1},\gamma_{2,1}} L(\gamma_{1,1},\gamma_{2,1},\lambda) \ &= \  \sigma_{1,1} \gamma_{1,1} + \delta \Bigg[ \frac{\sigma_{1,2}^2}{\sigma_{1,1}}  \gamma_{1,1} + \sqrt{\sigma_{2,2}^2 - \Big( \frac{\sigma_{1,2}^2}{\sigma_{1,1}} \Big)^2} \gamma_{2,1}   \Bigg] \\
\ &+ \ \lambda \big(1 - \gamma_{1,1}^2 - \gamma_{2,1}^2 \big)
\end{aligned}
\end{eqnarray}
First order conditions are
\begin{eqnarray}\label{eq:foc_gam11}
\frac{\partial L(\gamma_{1,1},\gamma_{2,1},\lambda) }{\partial \gamma_{1,1}} = \sigma_{1,1} + \delta\frac{\sigma_{1,2}^2}{\sigma_{1,1}} - 2 \lambda \big( \gamma_{1,1}^* \big)^2 = 0 \ \ \Rightarrow \ \ \gamma_{1,1}^* = \frac{1}{2 \lambda} \bigg[ \sigma_{1,1} +  \delta\frac{\sigma_{1,2}^2}{\sigma_{1,1}}  \bigg]
\end{eqnarray}
\begin{eqnarray}\label{eq:foc_gam21}
\frac{\partial L(\gamma_{1,1},\gamma_{2,1},\lambda) }{\partial \gamma_{2,1}} = \delta \sqrt{\sigma_{2,2}^2 - \Big( \frac{\sigma_{1,2}^2}{\sigma_{1,1}} \Big)^2} - 2 \lambda \big( \gamma_{2,1}^* \big)^2 = 0 \ \ \Rightarrow \ \ \gamma_{2,1}^* =  \frac{1}{2 \lambda} \delta \sqrt{\sigma_{2,2}^2 - \Big( \frac{\sigma_{1,2}^2}{\sigma_{1,1}} \Big)^2}
\end{eqnarray}
\begin{eqnarray}\label{eq:complslackness}
\lambda \frac{\partial L(\gamma_{1,1},\gamma_{2,1},\lambda) }{\partial \lambda} = \lambda\big[ 1 - \big( \gamma_{1,1}^* \big)^2 - \big( \gamma_{2,1}^* \big)^2 \big] = 0
\end{eqnarray}
where $\lambda \geq 0$.

\

\begin{itemize}
\item Equation \ref{eq:foc_gam11} implies that
\begin{enumerate}
	\item $\gamma_{1,1}^* \geq 0$ for all $\delta \geq 0$ if $\sigma_{1,2}^2 \geq 0$.
	\item It exists $\bar{\delta}$ such that $\gamma_{1,1}^* \geq 0$ for all $0 \leq \delta \leq \bar{\delta}$ if $\sigma_{1,2}^2 \leq 0$.
\end{enumerate} 

\item Equation \ref{eq:foc_gam21} implies $\gamma_{2,1}^* \geq 0$ for all $\delta \geq 0$.

\item Dividing \ref{eq:foc_gam11} over \ref{eq:foc_gam21} yields
$$
\frac{\gamma_{1,1}^*}{\gamma_{2,1}^*} = \frac{\sigma_{1,1} + \delta \frac{\sigma_{1,2}^2}{\sigma_{1,1}}}{\delta \sqrt{\sigma_{2,2} - \Big(\frac{\sigma_{1,1}^2}{\sigma_11}\Big)^2}} 
$$
Taking first derivative with respect to $\delta$ implies
$$
\frac{\partial \frac{\gamma_{1,1}^*}{\gamma_{2,1}^*}}{\partial \delta} = \frac{\frac{\sigma_{1,2}^2}{\sigma_{1,1}} \delta  \sqrt{\sigma_{2,2} - \Big(\frac{\sigma_{1,1}^2}{\sigma_11}\Big)^2}    - \Big( \sigma_{1,1} + \delta \frac{\sigma_{1,2}^2}{\sigma_{1,1}}  \Big)  \sqrt{\sigma_{2,2} - \Big(\frac{\sigma_{1,1}^2}{\sigma_11}\Big)^2}  }{\delta^2 \Big(   \sigma_{2,2} - \Big(\frac{\sigma_{1,1}^2}{\sigma_11}\Big)^2  \Big)}
$$ 
\end{itemize}
}


\end{document}